src/Stringification/Java.v
@@ -1,0 +1,379 @@
+From Coq Require Import ZArith.ZArith MSets.MSetPositive FSets.FMapPositive
+     Strings.String Strings.Ascii Bool.Bool Lists.List.
+From Crypto.Util Require Import
+     ListUtil
+     Strings.String Strings.Decimal Strings.HexString Strings.Show
+     ZRange ZRange.Operations ZRange.Show
+     Option OptionList Bool.Equality.
+
+From Crypto Require Import IR Stringification.Language AbstractInterpretation.
+
+Import ListNotations.
+
+Local Open Scope string_scope.
+Local Open Scope list_scope.
+Local Open Scope zrange_scope.
+Local Open Scope Z_scope.
+
+Module IR := IR.Compilers.ToString.IR.
+Module ToString := Stringification.Language.Compilers.ToString.
+Import Stringification.Language.Compilers.Options.
+
+Module Java.
+
+  (* Header imports and type defs *)
+  Definition header (static : bool) (prefix : string) (infos : ToString.ident_infos)
+  : list string
+    (* N.B. We don't do anything with static; we always export everything *)
+    := let bitwidths_used := ToString.bitwidths_used infos in
+       (* Java class names are in mixed case *)
+       let class_name := String.replace " " "" (String.to_title_case (String.replace "_" " " prefix)) in
+       ((["package fiat_crypto;";
+         "";
+         "public final class " ++ class_name ++ " {";
+         (** Java doesn't have pointers, so we make them *)
+         "";
+         "static class Box<T> {";
+         "  private T value;";
+         "  public Box(T value) { this.value = value; }";
+         "  public void set(T value) { this.value = value; }";
+         "  public T get() { return this.value; }";
+         "}";
+         ""]%string)).
+  Definition footer (static : bool) (prefix : string) (infos : ToString.ident_infos)
+    : list string
+    := ["}"]%string.
+
+  (* Supported integer bitwidths *)
+  Definition stdint_bitwidths : list Z := [32; 64].
+  Definition is_special_bitwidth (bw : Z) := negb (existsb (Z.eqb bw) stdint_bitwidths).
+
+
+  Definition int_type_to_string (use_class : bool) (prefix : string) (t : ToString.int.type) : string :=
+    let bw := ToString.int.bitwidth_of t in
+    if bw =? 1 (* we have some of these left over from carries guaranteed to be 0; we use int for them because that's the only thing that will typecheck.  This is a bit of a kludge *)
+    then if use_class then "Integer" else "int"
+    else if bw =? 8 then if use_class then "Byte" else "byte"
+         else if bw =? 16 then if use_class then "Short" else "short"
+              else if bw =? 32 then if use_class then "Integer" else "int"
+                   else if bw =? 64 then if use_class then "Long" else "long"
+                        else (prefix
+                                ++ (if ToString.int.is_unsigned t then "uint" else "int")
+                                ++ decimal_string_of_Z (ToString.int.bitwidth_of t))%string.
+
+  Definition primitive_type_to_string (use_class : bool) (prefix : string) (t : IR.type.primitive)
+             (r : option ToString.int.type) : string :=
+    match t with
+    | IR.type.Zptr => fun t => "Box<" ++ t true ++">"
+    | IR.type.Z => fun t => t use_class
+    end%string
+       (fun use_class
+        => match r with
+           | Some int_t => int_type_to_string use_class prefix int_t
+           | None => "ℤ" (* blackboard bold Z for unbounded integers (which don't actually exist, and thus will error) *)
+           end).
+
+  (* Integer literal to string *)
+  Definition int_literal_to_string (prefix : string) (t : IR.type.primitive) (v : BinInt.Z) : string :=
+    match t with
+    | IR.type.Z
+      => (HexString.of_Z v)
+           ++ if ToString.int.bitwidth_of (ToString.int.of_zrange_relaxed r[v ~> v]) >? 32
+              then "L"
+              else ""
+    | IR.type.Zptr => "error_literal_address_" ++ HexString.of_Z v
+    end%string.
+
+  Import IR.Notations.
+
+  Fixpoint arith_to_string (prefix : string) {t} (e : IR.arith_expr t) : string
+    := match e with
+       (* integer literals *)
+       | (IR.literal v @@ _) => int_literal_to_string prefix IR.type.Z v
+       (* array dereference *)
+       | (IR.List_nth n @@ IR.Var _ v) => "(" ++ v ++ "[" ++ decimal_string_of_Z (Z.of_nat n) ++ "])"
+       (* (de)referencing *)
+       | (IR.Dereference @@ e) => "(" ++ arith_to_string prefix e ++ ").get()"
+       (* bitwise operations *)
+       | (IR.Z_shiftr offset @@ e) =>
+         (* We assume that shift is always unsigned *)
+         "(" ++ arith_to_string prefix e ++ " >>> " ++ decimal_string_of_Z offset ++ ")"
+       | (IR.Z_shiftl offset @@ e) =>
+         "(" ++ arith_to_string prefix e ++ " << " ++ decimal_string_of_Z offset ++ ")"
+       | (IR.Z_land @@ (e1, e2)) =>
+         "(" ++ arith_to_string prefix e1 ++ " & " ++ arith_to_string prefix e2 ++ ")"
+       | (IR.Z_lor @@ (e1, e2)) =>
+         "(" ++ arith_to_string prefix e1 ++ " | " ++ arith_to_string prefix e2 ++ ")"
+       | (IR.Z_lnot _ @@ e) => "(~" ++ arith_to_string prefix e ++ ")"
+       (* arithmetic operations *)
+       | (IR.Z_add @@ (x1, x2)) =>
+         "(" ++ arith_to_string prefix x1 ++ " + " ++ arith_to_string prefix x2 ++ ")"
+       | (IR.Z_mul @@ (x1, x2)) =>
+         "(" ++ arith_to_string prefix x1 ++ " * " ++ arith_to_string prefix x2 ++ ")"
+       | (IR.Z_sub @@ (x1, x2)) =>
+         "(" ++ arith_to_string prefix x1 ++ " - " ++ arith_to_string prefix x2 ++ ")"
+       | (IR.Z_bneg @@ e) => "(!/* TODO: FIX ME */ " ++ arith_to_string prefix e ++ ")"
+       | (IR.Z_mul_split lg2s @@ args) =>
+         prefix
+           ++ "mulx_u"
+           ++ decimal_string_of_Z lg2s ++ "(" ++ arith_to_string prefix args ++ ")"
+       | (IR.Z_add_with_get_carry lg2s @@ args) =>
+         prefix
+           ++ "addcarryx_u"
+           ++ decimal_string_of_Z lg2s ++ "(" ++ arith_to_string prefix args ++ ")"
+       | (IR.Z_sub_with_get_borrow lg2s @@ args) =>
+         prefix
+           ++ "subborrowx_u"
+           ++ decimal_string_of_Z lg2s ++ "(" ++ arith_to_string prefix args ++ ")"
+       | (IR.Z_zselect ty @@ args) =>
+         prefix
+           ++ "cmovznz_u"
+           ++ decimal_string_of_Z (ToString.int.bitwidth_of ty) ++ "(" ++ @arith_to_string prefix _ args ++ ")"
+       | (IR.Z_static_cast int_t @@ e) =>
+         "Long.valueOf(" ++ arith_to_string prefix e ++ ")." ++ primitive_type_to_string false prefix IR.type.Z (Some int_t) ++ "Value()"
+       | IR.Var _ v => v
+       | IR.Pair A B a b => arith_to_string prefix a ++ ", " ++ arith_to_string prefix b
+       | (IR.Addr @@ IR.Var _ v) => "error_cannot_take_reference_in_Java_to_" ++ v
+       | (IR.Z_add_modulo @@ (x1, x2, x3)) => "int _error = error_addmodulo"
+       | (IR.List_nth _ @@ _)
+       | (IR.Addr @@ _)
+       | (IR.Z_add @@ _)
+       | (IR.Z_mul @@ _)
+       | (IR.Z_sub @@ _)
+       | (IR.Z_land @@ _)
+       | (IR.Z_lor @@ _)
+       | (IR.Z_add_modulo @@ _) => "int _error = error_bad_arg"
+       | TT => "error_tt"
+       end%string%Cexpr.
+
+  (** In Java, there is no munging of return arguments (they remain
+      passed by pointers), so all variables are live *)
+  Local Instance : IR.OfPHOAS.consider_retargs_live_opt := fun _ _ _ => true.
+  Local Instance : IR.OfPHOAS.rename_dead_opt := fun s => s.
+
+  Fixpoint stmt_to_string (prefix : string) (e : IR.stmt) : string :=
+    match e with
+    | IR.Call val => arith_to_string prefix val ++ ";"
+    | IR.Assign true t sz name val =>
+      (* local non-mutable declaration with initialization *)
+      primitive_type_to_string false prefix t sz ++ " " ++ name ++ " = " ++ arith_to_string prefix val ++ ";"
+    | IR.Assign false _ sz name val =>
+    (* This corresponds to assignment to a non-pointer variable and should never ever
+       happen in our generated code. Fiat-crypto handles it but I
+       haven't found and instance of this to their generated code *)
+    (* code : name ++ " = " ++ arith_to_string prefix val ++ ";" *)
+      "error_trying_to_assign_value_to_non_mutable_variable;"
+    | IR.AssignZPtr name sz val =>
+      name ++ ".set(" ++ arith_to_string prefix val ++ ");"
+    | IR.DeclareVar t sz name =>
+      (* Local uninitialized declarations become mut declarations, and
+         are initialized to 0. *)
+      (* The assumptions here, based on fiat-crypto code generation
+         patterns, are that 1.) this variable will be an argument to a
+         call that will store its result in this variable. 2.) this will
+         have a non-pointer an integer type *)
+      primitive_type_to_string true prefix IR.type.Zptr sz ++ " " ++ name ++ " = new " ++ primitive_type_to_string true prefix IR.type.Zptr sz ++ "((" ++ primitive_type_to_string false prefix IR.type.Z sz ++ ")0);"
+    | IR.AssignNth name n val =>
+      name ++ "[" ++ decimal_string_of_Z (Z.of_nat n) ++ "] = " ++ arith_to_string prefix val ++ ";"
+    end.
+
+  Definition to_strings (prefix : string) (e : IR.expr) : list string :=
+    List.map (stmt_to_string prefix) e.
+
+  Import Rewriter.Language.Language.Compilers Crypto.Language.API.Compilers IR.OfPHOAS.
+  Local Notation tZ := (base.type.type_base base.type.Z).
+
+  Inductive Mode := In | Out.
+
+
+  (* This would have been nice, but coercions don't work *)
+  (* Module Base := Rewriter.Language.Language.Compilers.base. *)
+
+  Fixpoint to_base_arg_list (prefix : string) (mode : Mode) {t} : ToString.OfPHOAS.base_var_data t -> list string :=
+    match t return base_var_data t -> _ with
+    | tZ =>
+      let typ := match mode with In => IR.type.Z | Out => IR.type.Zptr end in
+      fun '(n, is_ptr, r) => [primitive_type_to_string false prefix typ r ++ " " ++ n]
+    | base.type.prod A B =>
+      fun '(va, vb) => (to_base_arg_list prefix mode va ++ to_base_arg_list prefix mode vb)%list
+    | base.type.list tZ =>
+      fun '(n, r, len) =>
+        match mode with
+        | In => (* arrays for inputs are immutable borrows *)
+          [("final " ++ primitive_type_to_string false prefix IR.type.Z r)
+             ++ "[] " (* ++ decimal_string_of_Z (Z.of_nat len) ++ "] "*)
+             ++ n]
+        | Out => (* arrays for outputs are mutable borrows *)
+          [(primitive_type_to_string false prefix IR.type.Z r)
+             ++ "[] " (* ++ decimal_string_of_Z (Z.of_nat len) ++ "] "*)
+             ++ n]
+        end
+    | base.type.list _ => fun _ => ["error_complex_list"]
+    | base.type.option _ => fun _ => ["error_option"]
+    | base.type.unit => fun _ => ["error_unit"]
+    | base.type.type_base t => fun _ => ["error_" ++ show false t]%string
+    end%string.
+
+  Definition to_arg_list (prefix : string) (mode : Mode) {t} : var_data t -> list string :=
+    match t return var_data t -> _ with
+    | type.base t => to_base_arg_list prefix mode
+    | type.arrow _ _ => fun _ => ["error_arrow"]
+    end%string.
+
+  Fixpoint to_arg_list_for_each_lhs_of_arrow (prefix : string) {t} : type.for_each_lhs_of_arrow var_data t -> list string
+    := match t return type.for_each_lhs_of_arrow var_data t -> _ with
+       | type.base t => fun _ => nil
+       | type.arrow s d
+         => fun '(x, xs)
+            => to_arg_list prefix In x ++ @to_arg_list_for_each_lhs_of_arrow prefix d xs
+       end%list.
+
+  (** * Language-specific numeric conversions to be passed to the PHOAS -> IR translation *)
+
+  Definition Java_bin_op_natural_output
+    : IR.Z_binop -> ToString.int.type * ToString.int.type -> ToString.int.type
+    := fun idc '(t1, t2)
+       => ToString.int.union t1 t2.
+
+  (* Does the binary operation commute with (-- mod 2^bw)? *)
+  Definition bin_op_commutes_with_mod_pow2 (idc : IR.Z_binop)
+    := match idc with
+       | IR.Z_land
+       | IR.Z_lor
+       | IR.Z_add
+       | IR.Z_mul
+       | IR.Z_sub
+         => true
+       end.
+
+  Definition Java_bin_op_casts
+    : IR.Z_binop -> option ToString.int.type -> ToString.int.type * ToString.int.type -> option ToString.int.type * (option ToString.int.type * option ToString.int.type)
+    := fun idc desired_type '(t1, t2)
+       => match desired_type with
+          | Some desired_type
+            => let ct := ToString.int.union t1 t2 in
+               if bin_op_commutes_with_mod_pow2 idc
+               then
+                 (* these operations commute with mod, so we just pre-cast them *)
+                 (None, (Some desired_type, Some desired_type))
+               else
+                 let desired_type' := Some (ToString.int.union ct desired_type) in
+                 (desired_type',
+                  (get_Zcast_up_if_needed desired_type' (Some t1),
+                   get_Zcast_up_if_needed desired_type' (Some t2)))
+          | None => (None, (None, None))
+          end.
+
+  Definition Java_un_op_casts
+    : IR.Z_unop -> option ToString.int.type -> ToString.int.type -> option ToString.int.type * option ToString.int.type
+    := fun idc desired_type t
+       => match idc with
+          | IR.Z_shiftr offset
+            => (** N.B. We must cast the expression up to a large
+                   enough type to fit 2^offset (importantly, not just
+                   2^offset-1), because C considers it to be undefined
+                   behavior to shift >= width of the type.  We should
+                   probably figure out how to not generate these
+                   things in the first place...
+
+                   N.B. We must preserve signedness of the value being
+                   shifted, because shift does not commute with
+                   mod. *)
+            let t' := ToString.int.union_zrange r[0~>2^offset]%zrange t in
+            ((** We cast the result down to the specified type, if needed *)
+              get_Zcast_down_if_needed desired_type (Some t'),
+              (** We cast the argument up to a large enough type *)
+              get_Zcast_up_if_needed (Some t') (Some t))
+          | IR.Z_shiftl offset
+            => (** N.B. We must cast the expression up to a large
+                   enough type to fit 2^offset (importantly, not just
+                   2^offset-1), because C considers it to be undefined
+                   behavior to shift >= width of the type.  We should
+                   probably figure out how to not generate these
+                   things in the first place...
+
+                   N.B. We make sure that we only left-shift unsigned
+                   values, since shifting into the sign bit is
+                   undefined behavior. *)
+            let rpre_out := match desired_type with
+                            | Some rout => Some (ToString.int.union_zrange r[0~>2^offset] (ToString.int.unsigned_counterpart_of rout))
+                            | None => Some (ToString.int.of_zrange_relaxed r[0~>2^offset]%zrange)
+                            end in
+            ((** We cast the result down to the specified type, if needed *)
+              get_Zcast_down_if_needed desired_type rpre_out,
+              (** We cast the argument up to a large enough type *)
+              get_Zcast_up_if_needed rpre_out (Some t))
+          | IR.Z_lnot ty
+            => ((* if the result is too big, we cast it down; we
+                       don't need to upcast it because it'll get
+                       picked up by implicit casts if necessary *)
+              get_Zcast_down_if_needed desired_type (Some ty),
+              (** always cast to the width of the type, unless we are already exactly that type (which the machinery in IR handles *)
+              Some ty)
+          | Z_bneg
+            => ((* bneg is !, i.e., takes the argument to 1 if its not zero, and to zero if it is zero; so we don't ever need to cast *)
+              None, None)
+          end.
+
+  Local Instance JavaLanguageCasts : LanguageCasts :=
+    {| bin_op_natural_output := Java_bin_op_natural_output
+       ; bin_op_casts := Java_bin_op_casts
+       ; un_op_casts := Java_un_op_casts
+       ; upcast_on_assignment := true
+       ; upcast_on_funcall := true
+       ; explicit_pointer_variables := true (* Java can't take the address of a variable, so we declare explicit pointer variables *)
+    |}.
+
+  Definition to_function_lines (internal : bool) (prefix : string) (name : string)
+             {t}
+             (f : type.for_each_lhs_of_arrow var_data t * var_data (type.base (type.final_codomain t)) * IR.expr)
+    : list string :=
+    let '(args, rets, body) := f in
+    (((if internal then "" else "public ") ++ "static void " ++ name)
+       ++ "(" ++ String.concat ", " (to_arg_list prefix Out rets ++ to_arg_list_for_each_lhs_of_arrow prefix args) ++
+       ") {")%string :: (List.map (fun s => "  " ++ s)%string (to_strings prefix body)) ++ ["}"%string]%list.
+
+  Definition javadoc_replace (s : string) : string
+    := String.replace "<" "&lt;" (String.replace ">" "&gt;" s).
+
+  Definition javadoc_format (ls : list string) : list string
+    := ["/**"%string]
+         ++ List.map (fun s => s ++ " <p>")%string ls
+         ++ [" */"%string].
+
+  Definition ToFunctionLines
+             {relax_zrange : relax_zrange_opt}
+             (do_bounds_check : bool) (internal : bool) (prefix : string) (name : string)
+             {t}
+             (e : API.Expr t)
+             (comment : type.for_each_lhs_of_arrow var_data t -> var_data (type.base (type.final_codomain t)) -> list string)
+             (name_list : option (list string))
+             (inbounds : type.for_each_lhs_of_arrow Compilers.ZRange.type.option.interp t)
+             (outbounds : Compilers.ZRange.type.base.option.interp (type.final_codomain t))
+    : (list string * ToString.ident_infos) + string :=
+    match ExprOfPHOAS do_bounds_check e name_list inbounds with
+    | inl (indata, outdata, f) =>
+      inl ((javadoc_format
+              ((List.map (fun s => if (String.length s =? 0)%nat then " *" else (" * " ++ javadoc_replace s))%string (comment indata outdata))
+                 ++ [" * Input Bounds:"%string]
+                 ++ List.map (fun v => " *   "%string ++ javadoc_replace v)%string (input_bounds_to_string indata inbounds)
+                 ++ [" * Output Bounds:"%string]
+                 ++ List.map (fun v => " *   "%string ++ javadoc_replace v)%string (bound_to_string outdata outbounds))
+              ++ to_function_lines internal prefix name (indata, outdata, f))%list,
+           IR.ident_infos.collect_infos f)
+    | inr nil =>
+      inr ("Unknown internal error in converting " ++ name ++ " to Java")%string
+    | inr [err] =>
+      inr ("Error in converting " ++ name ++ " to Java:" ++ String.NewLine ++ err)%string
+    | inr errs =>
+      inr ("Errors in converting " ++ name ++ " to Java:" ++ String.NewLine ++ String.concat String.NewLine errs)%string
+    end.
+
+  Definition OutputJavaAPI : ToString.OutputLanguageAPI :=
+    {| ToString.comment_block := List.map (fun line => "/* " ++ line ++ " */")%string;
+       ToString.ToFunctionLines := @ToFunctionLines;
+       ToString.header := header;
+       ToString.footer := footer;
+       ToString.strip_special_infos infos := infos |}.
+
+End Java.
